tests

examples/pipeline_tutorial.v
@@ -30,7 +30,544 @@ Inductive reg_t :=
 | input_buffer (** The data source (from which we read inputs) *)
 | queue_empty (** A flag indicating whether the queue is empty *)
 | queue_data (** The data stored in the queue *)
-| output_buffer. (** The data sink (into which we write outputs) *)
+| output_buffer (** The data sink (into which we write outputs) *)
+| output_buffer_1 (** The data sink (into which we write outputs) *)
+| output_buffer_2 (** The data sink (into which we write outputs) *)
+| output_buffer_3 (** The data sink (into which we write outputs) *)
+| output_buffer_4 (** The data sink (into which we write outputs) *)
+| output_buffer_5 (** The data sink (into which we write outputs) *)
+| output_buffer_6 (** The data sink (into which we write outputs) *)
+| output_buffer_7 (** The data sink (into which we write outputs) *)
+| output_buffer_8 (** The data sink (into which we write outputs) *)
+| output_buffer_9 (** The data sink (into which we write outputs) *)
+| output_buffer_10 (** The data sink (into which we write outputs) *)
+| output_buffer_11 (** The data sink (into which we write outputs) *)
+| output_buffer_12 (** The data sink (into which we write outputs) *)
+| output_buffer_13 (** The data sink (into which we write outputs) *)
+| output_buffer_14 (** The data sink (into which we write outputs) *)
+| output_buffer_15 (** The data sink (into which we write outputs) *)
+| output_buffer_16 (** The data sink (into which we write outputs) *)
+| output_buffer_17 (** The data sink (into which we write outputs) *)
+| output_buffer_18 (** The data sink (into which we write outputs) *)
+| output_buffer_19 (** The data sink (into which we write outputs) *)
+| output_buffer_20 (** The data sink (into which we write outputs) *)
+| output_buffer_21 (** The data sink (into which we write outputs) *)
+| output_buffer_22 (** The data sink (into which we write outputs) *)
+| output_buffer_23 (** The data sink (into which we write outputs) *)
+| output_buffer_24 (** The data sink (into which we write outputs) *)
+| output_buffer_25 (** The data sink (into which we write outputs) *)
+| output_buffer_26 (** The data sink (into which we write outputs) *)
+| output_buffer_27 (** The data sink (into which we write outputs) *)
+| output_buffer_28 (** The data sink (into which we write outputs) *)
+| output_buffer_29 (** The data sink (into which we write outputs) *)
+| output_buffer_30 (** The data sink (into which we write outputs) *)
+| output_buffer_31 (** The data sink (into which we write outputs) *)
+| output_buffer_32 (** The data sink (into which we write outputs) *)
+| output_buffer_33 (** The data sink (into which we write outputs) *)
+| output_buffer_34 (** The data sink (into which we write outputs) *)
+| output_buffer_35 (** The data sink (into which we write outputs) *)
+| output_buffer_36 (** The data sink (into which we write outputs) *)
+| output_buffer_37 (** The data sink (into which we write outputs) *)
+| output_buffer_38 (** The data sink (into which we write outputs) *)
+| output_buffer_39 (** The data sink (into which we write outputs) *)
+| output_buffer_40 (** The data sink (into which we write outputs) *)
+| output_buffer_41 (** The data sink (into which we write outputs) *)
+| output_buffer_42 (** The data sink (into which we write outputs) *)
+| output_buffer_43 (** The data sink (into which we write outputs) *)
+| output_buffer_44 (** The data sink (into which we write outputs) *)
+| output_buffer_45 (** The data sink (into which we write outputs) *)
+| output_buffer_46 (** The data sink (into which we write outputs) *)
+| output_buffer_47 (** The data sink (into which we write outputs) *)
+| output_buffer_48 (** The data sink (into which we write outputs) *)
+| output_buffer_49 (** The data sink (into which we write outputs) *)
+| output_buffer_50 (** The data sink (into which we write outputs) *)
+| output_buffer_51 (** The data sink (into which we write outputs) *)
+| output_buffer_52 (** The data sink (into which we write outputs) *)
+| output_buffer_53 (** The data sink (into which we write outputs) *)
+| output_buffer_54 (** The data sink (into which we write outputs) *)
+| output_buffer_55 (** The data sink (into which we write outputs) *)
+| output_buffer_56 (** The data sink (into which we write outputs) *)
+| output_buffer_57 (** The data sink (into which we write outputs) *)
+| output_buffer_58 (** The data sink (into which we write outputs) *)
+| output_buffer_59 (** The data sink (into which we write outputs) *)
+| output_buffer_60 (** The data sink (into which we write outputs) *)
+| output_buffer_61 (** The data sink (into which we write outputs) *)
+| output_buffer_62 (** The data sink (into which we write outputs) *)
+| output_buffer_63 (** The data sink (into which we write outputs) *)
+| output_buffer_64 (** The data sink (into which we write outputs) *)
+| output_buffer_65 (** The data sink (into which we write outputs) *)
+| output_buffer_66 (** The data sink (into which we write outputs) *)
+| output_buffer_67 (** The data sink (into which we write outputs) *)
+| output_buffer_68 (** The data sink (into which we write outputs) *)
+| output_buffer_69 (** The data sink (into which we write outputs) *)
+| output_buffer_70 (** The data sink (into which we write outputs) *)
+| output_buffer_71 (** The data sink (into which we write outputs) *)
+| output_buffer_72 (** The data sink (into which we write outputs) *)
+| output_buffer_73 (** The data sink (into which we write outputs) *)
+| output_buffer_74 (** The data sink (into which we write outputs) *)
+| output_buffer_75 (** The data sink (into which we write outputs) *)
+| output_buffer_76 (** The data sink (into which we write outputs) *)
+| output_buffer_77 (** The data sink (into which we write outputs) *)
+| output_buffer_78 (** The data sink (into which we write outputs) *)
+| output_buffer_79 (** The data sink (into which we write outputs) *)
+| output_buffer_80 (** The data sink (into which we write outputs) *)
+| output_buffer_81 (** The data sink (into which we write outputs) *)
+| output_buffer_82 (** The data sink (into which we write outputs) *)
+| output_buffer_83 (** The data sink (into which we write outputs) *)
+| output_buffer_84 (** The data sink (into which we write outputs) *)
+| output_buffer_85 (** The data sink (into which we write outputs) *)
+| output_buffer_86 (** The data sink (into which we write outputs) *)
+| output_buffer_87 (** The data sink (into which we write outputs) *)
+| output_buffer_88 (** The data sink (into which we write outputs) *)
+| output_buffer_89 (** The data sink (into which we write outputs) *)
+| output_buffer_90 (** The data sink (into which we write outputs) *)
+| output_buffer_91 (** The data sink (into which we write outputs) *)
+| output_buffer_92 (** The data sink (into which we write outputs) *)
+| output_buffer_93 (** The data sink (into which we write outputs) *)
+| output_buffer_94 (** The data sink (into which we write outputs) *)
+| output_buffer_95 (** The data sink (into which we write outputs) *)
+| output_buffer_96 (** The data sink (into which we write outputs) *)
+| output_buffer_97 (** The data sink (into which we write outputs) *)
+| output_buffer_98 (** The data sink (into which we write outputs) *)
+| output_buffer_99 (** The data sink (into which we write outputs) *)
+| output_buffer_100 (** The data sink (into which we write outputs) *)
+| output_buffer_101 (** The data sink (into which we write outputs) *)
+| output_buffer_102 (** The data sink (into which we write outputs) *)
+| output_buffer_103 (** The data sink (into which we write outputs) *)
+| output_buffer_104 (** The data sink (into which we write outputs) *)
+| output_buffer_105 (** The data sink (into which we write outputs) *)
+| output_buffer_106 (** The data sink (into which we write outputs) *)
+| output_buffer_107 (** The data sink (into which we write outputs) *)
+| output_buffer_108 (** The data sink (into which we write outputs) *)
+| output_buffer_109 (** The data sink (into which we write outputs) *)
+| output_buffer_110 (** The data sink (into which we write outputs) *)
+| output_buffer_111 (** The data sink (into which we write outputs) *)
+| output_buffer_112 (** The data sink (into which we write outputs) *)
+| output_buffer_113 (** The data sink (into which we write outputs) *)
+| output_buffer_114 (** The data sink (into which we write outputs) *)
+| output_buffer_115 (** The data sink (into which we write outputs) *)
+| output_buffer_116 (** The data sink (into which we write outputs) *)
+| output_buffer_117 (** The data sink (into which we write outputs) *)
+| output_buffer_118 (** The data sink (into which we write outputs) *)
+| output_buffer_119 (** The data sink (into which we write outputs) *)
+| output_buffer_120 (** The data sink (into which we write outputs) *)
+| output_buffer_121 (** The data sink (into which we write outputs) *)
+| output_buffer_122 (** The data sink (into which we write outputs) *)
+| output_buffer_123 (** The data sink (into which we write outputs) *)
+| output_buffer_124 (** The data sink (into which we write outputs) *)
+| output_buffer_125 (** The data sink (into which we write outputs) *)
+| output_buffer_126 (** The data sink (into which we write outputs) *)
+| output_buffer_127 (** The data sink (into which we write outputs) *)
+| output_buffer_128 (** The data sink (into which we write outputs) *)
+| output_buffer_129 (** The data sink (into which we write outputs) *)
+| output_buffer_130 (** The data sink (into which we write outputs) *)
+| output_buffer_131 (** The data sink (into which we write outputs) *)
+| output_buffer_132 (** The data sink (into which we write outputs) *)
+| output_buffer_133 (** The data sink (into which we write outputs) *)
+| output_buffer_134 (** The data sink (into which we write outputs) *)
+| output_buffer_135 (** The data sink (into which we write outputs) *)
+| output_buffer_136 (** The data sink (into which we write outputs) *)
+| output_buffer_137 (** The data sink (into which we write outputs) *)
+| output_buffer_138 (** The data sink (into which we write outputs) *)
+| output_buffer_139 (** The data sink (into which we write outputs) *)
+| output_buffer_140 (** The data sink (into which we write outputs) *)
+| output_buffer_141 (** The data sink (into which we write outputs) *)
+| output_buffer_142 (** The data sink (into which we write outputs) *)
+| output_buffer_143 (** The data sink (into which we write outputs) *)
+| output_buffer_144 (** The data sink (into which we write outputs) *)
+| output_buffer_145 (** The data sink (into which we write outputs) *)
+| output_buffer_146 (** The data sink (into which we write outputs) *)
+| output_buffer_147 (** The data sink (into which we write outputs) *)
+| output_buffer_148 (** The data sink (into which we write outputs) *)
+| output_buffer_149 (** The data sink (into which we write outputs) *)
+| output_buffer_150 (** The data sink (into which we write outputs) *)
+| output_buffer_151 (** The data sink (into which we write outputs) *)
+| output_buffer_152 (** The data sink (into which we write outputs) *)
+| output_buffer_153 (** The data sink (into which we write outputs) *)
+| output_buffer_154 (** The data sink (into which we write outputs) *)
+| output_buffer_155 (** The data sink (into which we write outputs) *)
+| output_buffer_156 (** The data sink (into which we write outputs) *)
+| output_buffer_157 (** The data sink (into which we write outputs) *)
+| output_buffer_158 (** The data sink (into which we write outputs) *)
+| output_buffer_159 (** The data sink (into which we write outputs) *)
+| output_buffer_160 (** The data sink (into which we write outputs) *)
+| output_buffer_161 (** The data sink (into which we write outputs) *)
+| output_buffer_162 (** The data sink (into which we write outputs) *)
+| output_buffer_163 (** The data sink (into which we write outputs) *)
+| output_buffer_164 (** The data sink (into which we write outputs) *)
+| output_buffer_165 (** The data sink (into which we write outputs) *)
+| output_buffer_166 (** The data sink (into which we write outputs) *)
+| output_buffer_167 (** The data sink (into which we write outputs) *)
+| output_buffer_168 (** The data sink (into which we write outputs) *)
+| output_buffer_169 (** The data sink (into which we write outputs) *)
+| output_buffer_170 (** The data sink (into which we write outputs) *)
+| output_buffer_171 (** The data sink (into which we write outputs) *)
+| output_buffer_172 (** The data sink (into which we write outputs) *)
+| output_buffer_173 (** The data sink (into which we write outputs) *)
+| output_buffer_174 (** The data sink (into which we write outputs) *)
+| output_buffer_175 (** The data sink (into which we write outputs) *)
+| output_buffer_176 (** The data sink (into which we write outputs) *)
+| output_buffer_177 (** The data sink (into which we write outputs) *)
+| output_buffer_178 (** The data sink (into which we write outputs) *)
+| output_buffer_179 (** The data sink (into which we write outputs) *)
+| output_buffer_180 (** The data sink (into which we write outputs) *)
+| output_buffer_181 (** The data sink (into which we write outputs) *)
+| output_buffer_182 (** The data sink (into which we write outputs) *)
+| output_buffer_183 (** The data sink (into which we write outputs) *)
+| output_buffer_184 (** The data sink (into which we write outputs) *)
+| output_buffer_185 (** The data sink (into which we write outputs) *)
+| output_buffer_186 (** The data sink (into which we write outputs) *)
+| output_buffer_187 (** The data sink (into which we write outputs) *)
+| output_buffer_188 (** The data sink (into which we write outputs) *)
+| output_buffer_189 (** The data sink (into which we write outputs) *)
+| output_buffer_190 (** The data sink (into which we write outputs) *)
+| output_buffer_191 (** The data sink (into which we write outputs) *)
+| output_buffer_192 (** The data sink (into which we write outputs) *)
+| output_buffer_193 (** The data sink (into which we write outputs) *)
+| output_buffer_194 (** The data sink (into which we write outputs) *)
+| output_buffer_195 (** The data sink (into which we write outputs) *)
+| output_buffer_196 (** The data sink (into which we write outputs) *)
+| output_buffer_197 (** The data sink (into which we write outputs) *)
+| output_buffer_198 (** The data sink (into which we write outputs) *)
+| output_buffer_199 (** The data sink (into which we write outputs) *)
+| output_buffer_200 (** The data sink (into which we write outputs) *)
+| output_buffer_201 (** The data sink (into which we write outputs) *)
+| output_buffer_202 (** The data sink (into which we write outputs) *)
+| output_buffer_203 (** The data sink (into which we write outputs) *)
+| output_buffer_204 (** The data sink (into which we write outputs) *)
+| output_buffer_205 (** The data sink (into which we write outputs) *)
+| output_buffer_206 (** The data sink (into which we write outputs) *)
+| output_buffer_207 (** The data sink (into which we write outputs) *)
+| output_buffer_208 (** The data sink (into which we write outputs) *)
+| output_buffer_209 (** The data sink (into which we write outputs) *)
+| output_buffer_210 (** The data sink (into which we write outputs) *)
+| output_buffer_211 (** The data sink (into which we write outputs) *)
+| output_buffer_212 (** The data sink (into which we write outputs) *)
+| output_buffer_213 (** The data sink (into which we write outputs) *)
+| output_buffer_214 (** The data sink (into which we write outputs) *)
+| output_buffer_215 (** The data sink (into which we write outputs) *)
+| output_buffer_216 (** The data sink (into which we write outputs) *)
+| output_buffer_217 (** The data sink (into which we write outputs) *)
+| output_buffer_218 (** The data sink (into which we write outputs) *)
+| output_buffer_219 (** The data sink (into which we write outputs) *)
+| output_buffer_220 (** The data sink (into which we write outputs) *)
+| output_buffer_221 (** The data sink (into which we write outputs) *)
+| output_buffer_222 (** The data sink (into which we write outputs) *)
+| output_buffer_223 (** The data sink (into which we write outputs) *)
+| output_buffer_224 (** The data sink (into which we write outputs) *)
+| output_buffer_225 (** The data sink (into which we write outputs) *)
+| output_buffer_226 (** The data sink (into which we write outputs) *)
+| output_buffer_227 (** The data sink (into which we write outputs) *)
+| output_buffer_228 (** The data sink (into which we write outputs) *)
+| output_buffer_229 (** The data sink (into which we write outputs) *)
+| output_buffer_230 (** The data sink (into which we write outputs) *)
+| output_buffer_231 (** The data sink (into which we write outputs) *)
+| output_buffer_232 (** The data sink (into which we write outputs) *)
+| output_buffer_233 (** The data sink (into which we write outputs) *)
+| output_buffer_234 (** The data sink (into which we write outputs) *)
+| output_buffer_235 (** The data sink (into which we write outputs) *)
+| output_buffer_236 (** The data sink (into which we write outputs) *)
+| output_buffer_237 (** The data sink (into which we write outputs) *)
+| output_buffer_238 (** The data sink (into which we write outputs) *)
+| output_buffer_239 (** The data sink (into which we write outputs) *)
+| output_buffer_240 (** The data sink (into which we write outputs) *)
+| output_buffer_241 (** The data sink (into which we write outputs) *)
+| output_buffer_242 (** The data sink (into which we write outputs) *)
+| output_buffer_243 (** The data sink (into which we write outputs) *)
+| output_buffer_244 (** The data sink (into which we write outputs) *)
+| output_buffer_245 (** The data sink (into which we write outputs) *)
+| output_buffer_246 (** The data sink (into which we write outputs) *)
+| output_buffer_247 (** The data sink (into which we write outputs) *)
+| output_buffer_248 (** The data sink (into which we write outputs) *)
+| output_buffer_249 (** The data sink (into which we write outputs) *)
+| output_buffer_250 (** The data sink (into which we write outputs) *)
+| output_buffer_251 (** The data sink (into which we write outputs) *)
+| output_buffer_252 (** The data sink (into which we write outputs) *)
+| output_buffer_253 (** The data sink (into which we write outputs) *)
+| output_buffer_254 (** The data sink (into which we write outputs) *)
+| output_buffer_255 (** The data sink (into which we write outputs) *)
+| output_buffer_256 (** The data sink (into which we write outputs) *)
+| output_buffer_257 (** The data sink (into which we write outputs) *)
+| output_buffer_258 (** The data sink (into which we write outputs) *)
+| output_buffer_259 (** The data sink (into which we write outputs) *)
+| output_buffer_260 (** The data sink (into which we write outputs) *)
+| output_buffer_261 (** The data sink (into which we write outputs) *)
+| output_buffer_262 (** The data sink (into which we write outputs) *)
+| output_buffer_263 (** The data sink (into which we write outputs) *)
+| output_buffer_264 (** The data sink (into which we write outputs) *)
+| output_buffer_265 (** The data sink (into which we write outputs) *)
+| output_buffer_266 (** The data sink (into which we write outputs) *)
+| output_buffer_267 (** The data sink (into which we write outputs) *)
+| output_buffer_268 (** The data sink (into which we write outputs) *)
+| output_buffer_269 (** The data sink (into which we write outputs) *)
+| output_buffer_270 (** The data sink (into which we write outputs) *)
+| output_buffer_271 (** The data sink (into which we write outputs) *)
+| output_buffer_272 (** The data sink (into which we write outputs) *)
+| output_buffer_273 (** The data sink (into which we write outputs) *)
+| output_buffer_274 (** The data sink (into which we write outputs) *)
+| output_buffer_275 (** The data sink (into which we write outputs) *)
+| output_buffer_276 (** The data sink (into which we write outputs) *)
+| output_buffer_277 (** The data sink (into which we write outputs) *)
+| output_buffer_278 (** The data sink (into which we write outputs) *)
+| output_buffer_279 (** The data sink (into which we write outputs) *)
+| output_buffer_280 (** The data sink (into which we write outputs) *)
+| output_buffer_281 (** The data sink (into which we write outputs) *)
+| output_buffer_282 (** The data sink (into which we write outputs) *)
+| output_buffer_283 (** The data sink (into which we write outputs) *)
+| output_buffer_284 (** The data sink (into which we write outputs) *)
+| output_buffer_285 (** The data sink (into which we write outputs) *)
+| output_buffer_286 (** The data sink (into which we write outputs) *)
+| output_buffer_287 (** The data sink (into which we write outputs) *)
+| output_buffer_288 (** The data sink (into which we write outputs) *)
+| output_buffer_289 (** The data sink (into which we write outputs) *)
+| output_buffer_290 (** The data sink (into which we write outputs) *)
+| output_buffer_291 (** The data sink (into which we write outputs) *)
+| output_buffer_292 (** The data sink (into which we write outputs) *)
+| output_buffer_293 (** The data sink (into which we write outputs) *)
+| output_buffer_294 (** The data sink (into which we write outputs) *)
+| output_buffer_295 (** The data sink (into which we write outputs) *)
+| output_buffer_296 (** The data sink (into which we write outputs) *)
+| output_buffer_297 (** The data sink (into which we write outputs) *)
+| output_buffer_298 (** The data sink (into which we write outputs) *)
+| output_buffer_299 (** The data sink (into which we write outputs) *)
+| output_buffer_300 (** The data sink (into which we write outputs) *)
+| output_buffer_301 (** The data sink (into which we write outputs) *)
+| output_buffer_302 (** The data sink (into which we write outputs) *)
+| output_buffer_303 (** The data sink (into which we write outputs) *)
+| output_buffer_304 (** The data sink (into which we write outputs) *)
+| output_buffer_305 (** The data sink (into which we write outputs) *)
+| output_buffer_306 (** The data sink (into which we write outputs) *)
+| output_buffer_307 (** The data sink (into which we write outputs) *)
+| output_buffer_308 (** The data sink (into which we write outputs) *)
+| output_buffer_309 (** The data sink (into which we write outputs) *)
+| output_buffer_310 (** The data sink (into which we write outputs) *)
+| output_buffer_311 (** The data sink (into which we write outputs) *)
+| output_buffer_312 (** The data sink (into which we write outputs) *)
+| output_buffer_313 (** The data sink (into which we write outputs) *)
+| output_buffer_314 (** The data sink (into which we write outputs) *)
+| output_buffer_315 (** The data sink (into which we write outputs) *)
+| output_buffer_316 (** The data sink (into which we write outputs) *)
+| output_buffer_317 (** The data sink (into which we write outputs) *)
+| output_buffer_318 (** The data sink (into which we write outputs) *)
+| output_buffer_319 (** The data sink (into which we write outputs) *)
+| output_buffer_320 (** The data sink (into which we write outputs) *)
+| output_buffer_321 (** The data sink (into which we write outputs) *)
+| output_buffer_322 (** The data sink (into which we write outputs) *)
+| output_buffer_323 (** The data sink (into which we write outputs) *)
+| output_buffer_324 (** The data sink (into which we write outputs) *)
+| output_buffer_325 (** The data sink (into which we write outputs) *)
+| output_buffer_326 (** The data sink (into which we write outputs) *)
+| output_buffer_327 (** The data sink (into which we write outputs) *)
+| output_buffer_328 (** The data sink (into which we write outputs) *)
+| output_buffer_329 (** The data sink (into which we write outputs) *)
+| output_buffer_330 (** The data sink (into which we write outputs) *)
+| output_buffer_331 (** The data sink (into which we write outputs) *)
+| output_buffer_332 (** The data sink (into which we write outputs) *)
+| output_buffer_333 (** The data sink (into which we write outputs) *)
+| output_buffer_334 (** The data sink (into which we write outputs) *)
+| output_buffer_335 (** The data sink (into which we write outputs) *)
+| output_buffer_336 (** The data sink (into which we write outputs) *)
+| output_buffer_337 (** The data sink (into which we write outputs) *)
+| output_buffer_338 (** The data sink (into which we write outputs) *)
+| output_buffer_339 (** The data sink (into which we write outputs) *)
+| output_buffer_340 (** The data sink (into which we write outputs) *)
+| output_buffer_341 (** The data sink (into which we write outputs) *)
+| output_buffer_342 (** The data sink (into which we write outputs) *)
+| output_buffer_343 (** The data sink (into which we write outputs) *)
+| output_buffer_344 (** The data sink (into which we write outputs) *)
+| output_buffer_345 (** The data sink (into which we write outputs) *)
+| output_buffer_346 (** The data sink (into which we write outputs) *)
+| output_buffer_347 (** The data sink (into which we write outputs) *)
+| output_buffer_348 (** The data sink (into which we write outputs) *)
+| output_buffer_349 (** The data sink (into which we write outputs) *)
+| output_buffer_350 (** The data sink (into which we write outputs) *)
+| output_buffer_351 (** The data sink (into which we write outputs) *)
+| output_buffer_352 (** The data sink (into which we write outputs) *)
+| output_buffer_353 (** The data sink (into which we write outputs) *)
+| output_buffer_354 (** The data sink (into which we write outputs) *)
+| output_buffer_355 (** The data sink (into which we write outputs) *)
+| output_buffer_356 (** The data sink (into which we write outputs) *)
+| output_buffer_357 (** The data sink (into which we write outputs) *)
+| output_buffer_358 (** The data sink (into which we write outputs) *)
+| output_buffer_359 (** The data sink (into which we write outputs) *)
+| output_buffer_360 (** The data sink (into which we write outputs) *)
+| output_buffer_361 (** The data sink (into which we write outputs) *)
+| output_buffer_362 (** The data sink (into which we write outputs) *)
+| output_buffer_363 (** The data sink (into which we write outputs) *)
+| output_buffer_364 (** The data sink (into which we write outputs) *)
+| output_buffer_365 (** The data sink (into which we write outputs) *)
+| output_buffer_366 (** The data sink (into which we write outputs) *)
+| output_buffer_367 (** The data sink (into which we write outputs) *)
+| output_buffer_368 (** The data sink (into which we write outputs) *)
+| output_buffer_369 (** The data sink (into which we write outputs) *)
+| output_buffer_370 (** The data sink (into which we write outputs) *)
+| output_buffer_371 (** The data sink (into which we write outputs) *)
+| output_buffer_372 (** The data sink (into which we write outputs) *)
+| output_buffer_373 (** The data sink (into which we write outputs) *)
+| output_buffer_374 (** The data sink (into which we write outputs) *)
+| output_buffer_375 (** The data sink (into which we write outputs) *)
+| output_buffer_376 (** The data sink (into which we write outputs) *)
+| output_buffer_377 (** The data sink (into which we write outputs) *)
+| output_buffer_378 (** The data sink (into which we write outputs) *)
+| output_buffer_379 (** The data sink (into which we write outputs) *)
+| output_buffer_380 (** The data sink (into which we write outputs) *)
+| output_buffer_381 (** The data sink (into which we write outputs) *)
+| output_buffer_382 (** The data sink (into which we write outputs) *)
+| output_buffer_383 (** The data sink (into which we write outputs) *)
+| output_buffer_384 (** The data sink (into which we write outputs) *)
+| output_buffer_385 (** The data sink (into which we write outputs) *)
+| output_buffer_386 (** The data sink (into which we write outputs) *)
+| output_buffer_387 (** The data sink (into which we write outputs) *)
+| output_buffer_388 (** The data sink (into which we write outputs) *)
+| output_buffer_389 (** The data sink (into which we write outputs) *)
+| output_buffer_390 (** The data sink (into which we write outputs) *)
+| output_buffer_391 (** The data sink (into which we write outputs) *)
+| output_buffer_392 (** The data sink (into which we write outputs) *)
+| output_buffer_393 (** The data sink (into which we write outputs) *)
+| output_buffer_394 (** The data sink (into which we write outputs) *)
+| output_buffer_395 (** The data sink (into which we write outputs) *)
+| output_buffer_396 (** The data sink (into which we write outputs) *)
+| output_buffer_397 (** The data sink (into which we write outputs) *)
+| output_buffer_398 (** The data sink (into which we write outputs) *)
+| output_buffer_399 (** The data sink (into which we write outputs) *)
+| output_buffer_400 (** The data sink (into which we write outputs) *)
+| output_buffer_401 (** The data sink (into which we write outputs) *)
+| output_buffer_402 (** The data sink (into which we write outputs) *)
+| output_buffer_403 (** The data sink (into which we write outputs) *)
+| output_buffer_404 (** The data sink (into which we write outputs) *)
+| output_buffer_405 (** The data sink (into which we write outputs) *)
+| output_buffer_406 (** The data sink (into which we write outputs) *)
+| output_buffer_407 (** The data sink (into which we write outputs) *)
+| output_buffer_408 (** The data sink (into which we write outputs) *)
+| output_buffer_409 (** The data sink (into which we write outputs) *)
+| output_buffer_410 (** The data sink (into which we write outputs) *)
+| output_buffer_411 (** The data sink (into which we write outputs) *)
+| output_buffer_412 (** The data sink (into which we write outputs) *)
+| output_buffer_413 (** The data sink (into which we write outputs) *)
+| output_buffer_414 (** The data sink (into which we write outputs) *)
+| output_buffer_415 (** The data sink (into which we write outputs) *)
+| output_buffer_416 (** The data sink (into which we write outputs) *)
+| output_buffer_417 (** The data sink (into which we write outputs) *)
+| output_buffer_418 (** The data sink (into which we write outputs) *)
+| output_buffer_419 (** The data sink (into which we write outputs) *)
+| output_buffer_420 (** The data sink (into which we write outputs) *)
+| output_buffer_421 (** The data sink (into which we write outputs) *)
+| output_buffer_422 (** The data sink (into which we write outputs) *)
+| output_buffer_423 (** The data sink (into which we write outputs) *)
+| output_buffer_424 (** The data sink (into which we write outputs) *)
+| output_buffer_425 (** The data sink (into which we write outputs) *)
+| output_buffer_426 (** The data sink (into which we write outputs) *)
+| output_buffer_427 (** The data sink (into which we write outputs) *)
+| output_buffer_428 (** The data sink (into which we write outputs) *)
+| output_buffer_429 (** The data sink (into which we write outputs) *)
+| output_buffer_430 (** The data sink (into which we write outputs) *)
+| output_buffer_431 (** The data sink (into which we write outputs) *)
+| output_buffer_432 (** The data sink (into which we write outputs) *)
+| output_buffer_433 (** The data sink (into which we write outputs) *)
+| output_buffer_434 (** The data sink (into which we write outputs) *)
+| output_buffer_435 (** The data sink (into which we write outputs) *)
+| output_buffer_436 (** The data sink (into which we write outputs) *)
+| output_buffer_437 (** The data sink (into which we write outputs) *)
+| output_buffer_438 (** The data sink (into which we write outputs) *)
+| output_buffer_439 (** The data sink (into which we write outputs) *)
+| output_buffer_440 (** The data sink (into which we write outputs) *)
+| output_buffer_441 (** The data sink (into which we write outputs) *)
+| output_buffer_442 (** The data sink (into which we write outputs) *)
+| output_buffer_443 (** The data sink (into which we write outputs) *)
+| output_buffer_444 (** The data sink (into which we write outputs) *)
+| output_buffer_445 (** The data sink (into which we write outputs) *)
+| output_buffer_446 (** The data sink (into which we write outputs) *)
+| output_buffer_447 (** The data sink (into which we write outputs) *)
+| output_buffer_448 (** The data sink (into which we write outputs) *)
+| output_buffer_449 (** The data sink (into which we write outputs) *)
+| output_buffer_450 (** The data sink (into which we write outputs) *)
+| output_buffer_451 (** The data sink (into which we write outputs) *)
+| output_buffer_452 (** The data sink (into which we write outputs) *)
+| output_buffer_453 (** The data sink (into which we write outputs) *)
+| output_buffer_454 (** The data sink (into which we write outputs) *)
+| output_buffer_455 (** The data sink (into which we write outputs) *)
+| output_buffer_456 (** The data sink (into which we write outputs) *)
+| output_buffer_457 (** The data sink (into which we write outputs) *)
+| output_buffer_458 (** The data sink (into which we write outputs) *)
+| output_buffer_459 (** The data sink (into which we write outputs) *)
+| output_buffer_460 (** The data sink (into which we write outputs) *)
+| output_buffer_461 (** The data sink (into which we write outputs) *)
+| output_buffer_462 (** The data sink (into which we write outputs) *)
+| output_buffer_463 (** The data sink (into which we write outputs) *)
+| output_buffer_464 (** The data sink (into which we write outputs) *)
+| output_buffer_465 (** The data sink (into which we write outputs) *)
+| output_buffer_466 (** The data sink (into which we write outputs) *)
+| output_buffer_467 (** The data sink (into which we write outputs) *)
+| output_buffer_468 (** The data sink (into which we write outputs) *)
+| output_buffer_469 (** The data sink (into which we write outputs) *)
+| output_buffer_470 (** The data sink (into which we write outputs) *)
+| output_buffer_471 (** The data sink (into which we write outputs) *)
+| output_buffer_472 (** The data sink (into which we write outputs) *)
+| output_buffer_473 (** The data sink (into which we write outputs) *)
+| output_buffer_474 (** The data sink (into which we write outputs) *)
+| output_buffer_475 (** The data sink (into which we write outputs) *)
+| output_buffer_476 (** The data sink (into which we write outputs) *)
+| output_buffer_477 (** The data sink (into which we write outputs) *)
+| output_buffer_478 (** The data sink (into which we write outputs) *)
+| output_buffer_479 (** The data sink (into which we write outputs) *)
+| output_buffer_480 (** The data sink (into which we write outputs) *)
+| output_buffer_481 (** The data sink (into which we write outputs) *)
+| output_buffer_482 (** The data sink (into which we write outputs) *)
+| output_buffer_483 (** The data sink (into which we write outputs) *)
+| output_buffer_484 (** The data sink (into which we write outputs) *)
+| output_buffer_485 (** The data sink (into which we write outputs) *)
+| output_buffer_486 (** The data sink (into which we write outputs) *)
+| output_buffer_487 (** The data sink (into which we write outputs) *)
+| output_buffer_488 (** The data sink (into which we write outputs) *)
+| output_buffer_489 (** The data sink (into which we write outputs) *)
+| output_buffer_490 (** The data sink (into which we write outputs) *)
+| output_buffer_491 (** The data sink (into which we write outputs) *)
+| output_buffer_492 (** The data sink (into which we write outputs) *)
+| output_buffer_493 (** The data sink (into which we write outputs) *)
+| output_buffer_494 (** The data sink (into which we write outputs) *)
+| output_buffer_495 (** The data sink (into which we write outputs) *)
+| output_buffer_496 (** The data sink (into which we write outputs) *)
+| output_buffer_497 (** The data sink (into which we write outputs) *)
+| output_buffer_498 (** The data sink (into which we write outputs) *)
+| output_buffer_499 (** The data sink (into which we write outputs) *)
+| output_buffer_500 (** The data sink (into which we write outputs) *)
+| output_buffer_501 (** The data sink (into which we write outputs) *)
+| output_buffer_502 (** The data sink (into which we write outputs) *)
+| output_buffer_503 (** The data sink (into which we write outputs) *)
+| output_buffer_504 (** The data sink (into which we write outputs) *)
+| output_buffer_505 (** The data sink (into which we write outputs) *)
+| output_buffer_506 (** The data sink (into which we write outputs) *)
+| output_buffer_507 (** The data sink (into which we write outputs) *)
+| output_buffer_508 (** The data sink (into which we write outputs) *)
+| output_buffer_509 (** The data sink (into which we write outputs) *)
+| output_buffer_510 (** The data sink (into which we write outputs) *)
+| output_buffer_511 (** The data sink (into which we write outputs) *)
+| output_buffer_512 (** The data sink (into which we write outputs) *)
+| output_buffer_513 (** The data sink (into which we write outputs) *)
+| output_buffer_514 (** The data sink (into which we write outputs) *)
+| output_buffer_515 (** The data sink (into which we write outputs) *)
+| output_buffer_516 (** The data sink (into which we write outputs) *)
+| output_buffer_517 (** The data sink (into which we write outputs) *)
+| output_buffer_518 (** The data sink (into which we write outputs) *)
+| output_buffer_519 (** The data sink (into which we write outputs) *)
+| output_buffer_520 (** The data sink (into which we write outputs) *)
+| output_buffer_521 (** The data sink (into which we write outputs) *)
+| output_buffer_522 (** The data sink (into which we write outputs) *)
+| output_buffer_523 (** The data sink (into which we write outputs) *)
+| output_buffer_524 (** The data sink (into which we write outputs) *)
+| output_buffer_525 (** The data sink (into which we write outputs) *)
+| output_buffer_526 (** The data sink (into which we write outputs) *)
+| output_buffer_527 (** The data sink (into which we write outputs) *)
+| output_buffer_528 (** The data sink (into which we write outputs) *)
+| output_buffer_529 (** The data sink (into which we write outputs) *)
+| output_buffer_530 (** The data sink (into which we write outputs) *)
+| output_buffer_531 (** The data sink (into which we write outputs) *)
+| output_buffer_532 (** The data sink (into which we write outputs) *)
+| output_buffer_533 (** The data sink (into which we write outputs) *)
+| output_buffer_534 (** The data sink (into which we write outputs) *)
+| output_buffer_535 (** The data sink (into which we write outputs) *)
+| output_buffer_536 (** The data sink (into which we write outputs) *)
+.
 
 Definition R r :=
   match r with
@@ -38,6 +575,542 @@ Definition R r :=
   | queue_empty   => bits_t 1
   | queue_data    => bits_t sz
   | output_buffer => bits_t sz
+  | output_buffer_1 => bits_t sz
+  | output_buffer_2 => bits_t sz
+  | output_buffer_3 => bits_t sz
+  | output_buffer_4 => bits_t sz
+  | output_buffer_5 => bits_t sz
+  | output_buffer_6 => bits_t sz
+  | output_buffer_7 => bits_t sz
+  | output_buffer_8 => bits_t sz
+  | output_buffer_9 => bits_t sz
+  | output_buffer_10 => bits_t sz
+  | output_buffer_11 => bits_t sz
+  | output_buffer_12 => bits_t sz
+  | output_buffer_13 => bits_t sz
+  | output_buffer_14 => bits_t sz
+  | output_buffer_15 => bits_t sz
+  | output_buffer_16 => bits_t sz
+  | output_buffer_17 => bits_t sz
+  | output_buffer_18 => bits_t sz
+  | output_buffer_19 => bits_t sz
+  | output_buffer_20 => bits_t sz
+  | output_buffer_21 => bits_t sz
+  | output_buffer_22 => bits_t sz
+  | output_buffer_23 => bits_t sz
+  | output_buffer_24 => bits_t sz
+  | output_buffer_25 => bits_t sz
+  | output_buffer_26 => bits_t sz
+  | output_buffer_27 => bits_t sz
+  | output_buffer_28 => bits_t sz
+  | output_buffer_29 => bits_t sz
+  | output_buffer_30 => bits_t sz
+  | output_buffer_31 => bits_t sz
+  | output_buffer_32 => bits_t sz
+  | output_buffer_33 => bits_t sz
+  | output_buffer_34 => bits_t sz
+  | output_buffer_35 => bits_t sz
+  | output_buffer_36 => bits_t sz
+  | output_buffer_37 => bits_t sz
+  | output_buffer_38 => bits_t sz
+  | output_buffer_39 => bits_t sz
+  | output_buffer_40 => bits_t sz
+  | output_buffer_41 => bits_t sz
+  | output_buffer_42 => bits_t sz
+  | output_buffer_43 => bits_t sz
+  | output_buffer_44 => bits_t sz
+  | output_buffer_45 => bits_t sz
+  | output_buffer_46 => bits_t sz
+  | output_buffer_47 => bits_t sz
+  | output_buffer_48 => bits_t sz
+  | output_buffer_49 => bits_t sz
+  | output_buffer_50 => bits_t sz
+  | output_buffer_51 => bits_t sz
+  | output_buffer_52 => bits_t sz
+  | output_buffer_53 => bits_t sz
+  | output_buffer_54 => bits_t sz
+  | output_buffer_55 => bits_t sz
+  | output_buffer_56 => bits_t sz
+  | output_buffer_57 => bits_t sz
+  | output_buffer_58 => bits_t sz
+  | output_buffer_59 => bits_t sz
+  | output_buffer_60 => bits_t sz
+  | output_buffer_61 => bits_t sz
+  | output_buffer_62 => bits_t sz
+  | output_buffer_63 => bits_t sz
+  | output_buffer_64 => bits_t sz
+  | output_buffer_65 => bits_t sz
+  | output_buffer_66 => bits_t sz
+  | output_buffer_67 => bits_t sz
+  | output_buffer_68 => bits_t sz
+  | output_buffer_69 => bits_t sz
+  | output_buffer_70 => bits_t sz
+  | output_buffer_71 => bits_t sz
+  | output_buffer_72 => bits_t sz
+  | output_buffer_73 => bits_t sz
+  | output_buffer_74 => bits_t sz
+  | output_buffer_75 => bits_t sz
+  | output_buffer_76 => bits_t sz
+  | output_buffer_77 => bits_t sz
+  | output_buffer_78 => bits_t sz
+  | output_buffer_79 => bits_t sz
+  | output_buffer_80 => bits_t sz
+  | output_buffer_81 => bits_t sz
+  | output_buffer_82 => bits_t sz
+  | output_buffer_83 => bits_t sz
+  | output_buffer_84 => bits_t sz
+  | output_buffer_85 => bits_t sz
+  | output_buffer_86 => bits_t sz
+  | output_buffer_87 => bits_t sz
+  | output_buffer_88 => bits_t sz
+  | output_buffer_89 => bits_t sz
+  | output_buffer_90 => bits_t sz
+  | output_buffer_91 => bits_t sz
+  | output_buffer_92 => bits_t sz
+  | output_buffer_93 => bits_t sz
+  | output_buffer_94 => bits_t sz
+  | output_buffer_95 => bits_t sz
+  | output_buffer_96 => bits_t sz
+  | output_buffer_97 => bits_t sz
+  | output_buffer_98 => bits_t sz
+  | output_buffer_99 => bits_t sz
+  | output_buffer_100 => bits_t sz
+  | output_buffer_101 => bits_t sz
+  | output_buffer_102 => bits_t sz
+  | output_buffer_103 => bits_t sz
+  | output_buffer_104 => bits_t sz
+  | output_buffer_105 => bits_t sz
+  | output_buffer_106 => bits_t sz
+  | output_buffer_107 => bits_t sz
+  | output_buffer_108 => bits_t sz
+  | output_buffer_109 => bits_t sz
+  | output_buffer_110 => bits_t sz
+  | output_buffer_111 => bits_t sz
+  | output_buffer_112 => bits_t sz
+  | output_buffer_113 => bits_t sz
+  | output_buffer_114 => bits_t sz
+  | output_buffer_115 => bits_t sz
+  | output_buffer_116 => bits_t sz
+  | output_buffer_117 => bits_t sz
+  | output_buffer_118 => bits_t sz
+  | output_buffer_119 => bits_t sz
+  | output_buffer_120 => bits_t sz
+  | output_buffer_121 => bits_t sz
+  | output_buffer_122 => bits_t sz
+  | output_buffer_123 => bits_t sz
+  | output_buffer_124 => bits_t sz
+  | output_buffer_125 => bits_t sz
+  | output_buffer_126 => bits_t sz
+  | output_buffer_127 => bits_t sz
+  | output_buffer_128 => bits_t sz
+  | output_buffer_129 => bits_t sz
+  | output_buffer_130 => bits_t sz
+  | output_buffer_131 => bits_t sz
+  | output_buffer_132 => bits_t sz
+  | output_buffer_133 => bits_t sz
+  | output_buffer_134 => bits_t sz
+  | output_buffer_135 => bits_t sz
+  | output_buffer_136 => bits_t sz
+  | output_buffer_137 => bits_t sz
+  | output_buffer_138 => bits_t sz
+  | output_buffer_139 => bits_t sz
+  | output_buffer_140 => bits_t sz
+  | output_buffer_141 => bits_t sz
+  | output_buffer_142 => bits_t sz
+  | output_buffer_143 => bits_t sz
+  | output_buffer_144 => bits_t sz
+  | output_buffer_145 => bits_t sz
+  | output_buffer_146 => bits_t sz
+  | output_buffer_147 => bits_t sz
+  | output_buffer_148 => bits_t sz
+  | output_buffer_149 => bits_t sz
+  | output_buffer_150 => bits_t sz
+  | output_buffer_151 => bits_t sz
+  | output_buffer_152 => bits_t sz
+  | output_buffer_153 => bits_t sz
+  | output_buffer_154 => bits_t sz
+  | output_buffer_155 => bits_t sz
+  | output_buffer_156 => bits_t sz
+  | output_buffer_157 => bits_t sz
+  | output_buffer_158 => bits_t sz
+  | output_buffer_159 => bits_t sz
+  | output_buffer_160 => bits_t sz
+  | output_buffer_161 => bits_t sz
+  | output_buffer_162 => bits_t sz
+  | output_buffer_163 => bits_t sz
+  | output_buffer_164 => bits_t sz
+  | output_buffer_165 => bits_t sz
+  | output_buffer_166 => bits_t sz
+  | output_buffer_167 => bits_t sz
+  | output_buffer_168 => bits_t sz
+  | output_buffer_169 => bits_t sz
+  | output_buffer_170 => bits_t sz
+  | output_buffer_171 => bits_t sz
+  | output_buffer_172 => bits_t sz
+  | output_buffer_173 => bits_t sz
+  | output_buffer_174 => bits_t sz
+  | output_buffer_175 => bits_t sz
+  | output_buffer_176 => bits_t sz
+  | output_buffer_177 => bits_t sz
+  | output_buffer_178 => bits_t sz
+  | output_buffer_179 => bits_t sz
+  | output_buffer_180 => bits_t sz
+  | output_buffer_181 => bits_t sz
+  | output_buffer_182 => bits_t sz
+  | output_buffer_183 => bits_t sz
+  | output_buffer_184 => bits_t sz
+  | output_buffer_185 => bits_t sz
+  | output_buffer_186 => bits_t sz
+  | output_buffer_187 => bits_t sz
+  | output_buffer_188 => bits_t sz
+  | output_buffer_189 => bits_t sz
+  | output_buffer_190 => bits_t sz
+  | output_buffer_191 => bits_t sz
+  | output_buffer_192 => bits_t sz
+  | output_buffer_193 => bits_t sz
+  | output_buffer_194 => bits_t sz
+  | output_buffer_195 => bits_t sz
+  | output_buffer_196 => bits_t sz
+  | output_buffer_197 => bits_t sz
+  | output_buffer_198 => bits_t sz
+  | output_buffer_199 => bits_t sz
+  | output_buffer_200 => bits_t sz
+  | output_buffer_201 => bits_t sz
+  | output_buffer_202 => bits_t sz
+  | output_buffer_203 => bits_t sz
+  | output_buffer_204 => bits_t sz
+  | output_buffer_205 => bits_t sz
+  | output_buffer_206 => bits_t sz
+  | output_buffer_207 => bits_t sz
+  | output_buffer_208 => bits_t sz
+  | output_buffer_209 => bits_t sz
+  | output_buffer_210 => bits_t sz
+  | output_buffer_211 => bits_t sz
+  | output_buffer_212 => bits_t sz
+  | output_buffer_213 => bits_t sz
+  | output_buffer_214 => bits_t sz
+  | output_buffer_215 => bits_t sz
+  | output_buffer_216 => bits_t sz
+  | output_buffer_217 => bits_t sz
+  | output_buffer_218 => bits_t sz
+  | output_buffer_219 => bits_t sz
+  | output_buffer_220 => bits_t sz
+  | output_buffer_221 => bits_t sz
+  | output_buffer_222 => bits_t sz
+  | output_buffer_223 => bits_t sz
+  | output_buffer_224 => bits_t sz
+  | output_buffer_225 => bits_t sz
+  | output_buffer_226 => bits_t sz
+  | output_buffer_227 => bits_t sz
+  | output_buffer_228 => bits_t sz
+  | output_buffer_229 => bits_t sz
+  | output_buffer_230 => bits_t sz
+  | output_buffer_231 => bits_t sz
+  | output_buffer_232 => bits_t sz
+  | output_buffer_233 => bits_t sz
+  | output_buffer_234 => bits_t sz
+  | output_buffer_235 => bits_t sz
+  | output_buffer_236 => bits_t sz
+  | output_buffer_237 => bits_t sz
+  | output_buffer_238 => bits_t sz
+  | output_buffer_239 => bits_t sz
+  | output_buffer_240 => bits_t sz
+  | output_buffer_241 => bits_t sz
+  | output_buffer_242 => bits_t sz
+  | output_buffer_243 => bits_t sz
+  | output_buffer_244 => bits_t sz
+  | output_buffer_245 => bits_t sz
+  | output_buffer_246 => bits_t sz
+  | output_buffer_247 => bits_t sz
+  | output_buffer_248 => bits_t sz
+  | output_buffer_249 => bits_t sz
+  | output_buffer_250 => bits_t sz
+  | output_buffer_251 => bits_t sz
+  | output_buffer_252 => bits_t sz
+  | output_buffer_253 => bits_t sz
+  | output_buffer_254 => bits_t sz
+  | output_buffer_255 => bits_t sz
+  | output_buffer_256 => bits_t sz
+  | output_buffer_257 => bits_t sz
+  | output_buffer_258 => bits_t sz
+  | output_buffer_259 => bits_t sz
+  | output_buffer_260 => bits_t sz
+  | output_buffer_261 => bits_t sz
+  | output_buffer_262 => bits_t sz
+  | output_buffer_263 => bits_t sz
+  | output_buffer_264 => bits_t sz
+  | output_buffer_265 => bits_t sz
+  | output_buffer_266 => bits_t sz
+  | output_buffer_267 => bits_t sz
+  | output_buffer_268 => bits_t sz
+  | output_buffer_269 => bits_t sz
+  | output_buffer_270 => bits_t sz
+  | output_buffer_271 => bits_t sz
+  | output_buffer_272 => bits_t sz
+  | output_buffer_273 => bits_t sz
+  | output_buffer_274 => bits_t sz
+  | output_buffer_275 => bits_t sz
+  | output_buffer_276 => bits_t sz
+  | output_buffer_277 => bits_t sz
+  | output_buffer_278 => bits_t sz
+  | output_buffer_279 => bits_t sz
+  | output_buffer_280 => bits_t sz
+  | output_buffer_281 => bits_t sz
+  | output_buffer_282 => bits_t sz
+  | output_buffer_283 => bits_t sz
+  | output_buffer_284 => bits_t sz
+  | output_buffer_285 => bits_t sz
+  | output_buffer_286 => bits_t sz
+  | output_buffer_287 => bits_t sz
+  | output_buffer_288 => bits_t sz
+  | output_buffer_289 => bits_t sz
+  | output_buffer_290 => bits_t sz
+  | output_buffer_291 => bits_t sz
+  | output_buffer_292 => bits_t sz
+  | output_buffer_293 => bits_t sz
+  | output_buffer_294 => bits_t sz
+  | output_buffer_295 => bits_t sz
+  | output_buffer_296 => bits_t sz
+  | output_buffer_297 => bits_t sz
+  | output_buffer_298 => bits_t sz
+  | output_buffer_299 => bits_t sz
+  | output_buffer_300 => bits_t sz
+  | output_buffer_301 => bits_t sz
+  | output_buffer_302 => bits_t sz
+  | output_buffer_303 => bits_t sz
+  | output_buffer_304 => bits_t sz
+  | output_buffer_305 => bits_t sz
+  | output_buffer_306 => bits_t sz
+  | output_buffer_307 => bits_t sz
+  | output_buffer_308 => bits_t sz
+  | output_buffer_309 => bits_t sz
+  | output_buffer_310 => bits_t sz
+  | output_buffer_311 => bits_t sz
+  | output_buffer_312 => bits_t sz
+  | output_buffer_313 => bits_t sz
+  | output_buffer_314 => bits_t sz
+  | output_buffer_315 => bits_t sz
+  | output_buffer_316 => bits_t sz
+  | output_buffer_317 => bits_t sz
+  | output_buffer_318 => bits_t sz
+  | output_buffer_319 => bits_t sz
+  | output_buffer_320 => bits_t sz
+  | output_buffer_321 => bits_t sz
+  | output_buffer_322 => bits_t sz
+  | output_buffer_323 => bits_t sz
+  | output_buffer_324 => bits_t sz
+  | output_buffer_325 => bits_t sz
+  | output_buffer_326 => bits_t sz
+  | output_buffer_327 => bits_t sz
+  | output_buffer_328 => bits_t sz
+  | output_buffer_329 => bits_t sz
+  | output_buffer_330 => bits_t sz
+  | output_buffer_331 => bits_t sz
+  | output_buffer_332 => bits_t sz
+  | output_buffer_333 => bits_t sz
+  | output_buffer_334 => bits_t sz
+  | output_buffer_335 => bits_t sz
+  | output_buffer_336 => bits_t sz
+  | output_buffer_337 => bits_t sz
+  | output_buffer_338 => bits_t sz
+  | output_buffer_339 => bits_t sz
+  | output_buffer_340 => bits_t sz
+  | output_buffer_341 => bits_t sz
+  | output_buffer_342 => bits_t sz
+  | output_buffer_343 => bits_t sz
+  | output_buffer_344 => bits_t sz
+  | output_buffer_345 => bits_t sz
+  | output_buffer_346 => bits_t sz
+  | output_buffer_347 => bits_t sz
+  | output_buffer_348 => bits_t sz
+  | output_buffer_349 => bits_t sz
+  | output_buffer_350 => bits_t sz
+  | output_buffer_351 => bits_t sz
+  | output_buffer_352 => bits_t sz
+  | output_buffer_353 => bits_t sz
+  | output_buffer_354 => bits_t sz
+  | output_buffer_355 => bits_t sz
+  | output_buffer_356 => bits_t sz
+  | output_buffer_357 => bits_t sz
+  | output_buffer_358 => bits_t sz
+  | output_buffer_359 => bits_t sz
+  | output_buffer_360 => bits_t sz
+  | output_buffer_361 => bits_t sz
+  | output_buffer_362 => bits_t sz
+  | output_buffer_363 => bits_t sz
+  | output_buffer_364 => bits_t sz
+  | output_buffer_365 => bits_t sz
+  | output_buffer_366 => bits_t sz
+  | output_buffer_367 => bits_t sz
+  | output_buffer_368 => bits_t sz
+  | output_buffer_369 => bits_t sz
+  | output_buffer_370 => bits_t sz
+  | output_buffer_371 => bits_t sz
+  | output_buffer_372 => bits_t sz
+  | output_buffer_373 => bits_t sz
+  | output_buffer_374 => bits_t sz
+  | output_buffer_375 => bits_t sz
+  | output_buffer_376 => bits_t sz
+  | output_buffer_377 => bits_t sz
+  | output_buffer_378 => bits_t sz
+  | output_buffer_379 => bits_t sz
+  | output_buffer_380 => bits_t sz
+  | output_buffer_381 => bits_t sz
+  | output_buffer_382 => bits_t sz
+  | output_buffer_383 => bits_t sz
+  | output_buffer_384 => bits_t sz
+  | output_buffer_385 => bits_t sz
+  | output_buffer_386 => bits_t sz
+  | output_buffer_387 => bits_t sz
+  | output_buffer_388 => bits_t sz
+  | output_buffer_389 => bits_t sz
+  | output_buffer_390 => bits_t sz
+  | output_buffer_391 => bits_t sz
+  | output_buffer_392 => bits_t sz
+  | output_buffer_393 => bits_t sz
+  | output_buffer_394 => bits_t sz
+  | output_buffer_395 => bits_t sz
+  | output_buffer_396 => bits_t sz
+  | output_buffer_397 => bits_t sz
+  | output_buffer_398 => bits_t sz
+  | output_buffer_399 => bits_t sz
+  | output_buffer_400 => bits_t sz
+  | output_buffer_401 => bits_t sz
+  | output_buffer_402 => bits_t sz
+  | output_buffer_403 => bits_t sz
+  | output_buffer_404 => bits_t sz
+  | output_buffer_405 => bits_t sz
+  | output_buffer_406 => bits_t sz
+  | output_buffer_407 => bits_t sz
+  | output_buffer_408 => bits_t sz
+  | output_buffer_409 => bits_t sz
+  | output_buffer_410 => bits_t sz
+  | output_buffer_411 => bits_t sz
+  | output_buffer_412 => bits_t sz
+  | output_buffer_413 => bits_t sz
+  | output_buffer_414 => bits_t sz
+  | output_buffer_415 => bits_t sz
+  | output_buffer_416 => bits_t sz
+  | output_buffer_417 => bits_t sz
+  | output_buffer_418 => bits_t sz
+  | output_buffer_419 => bits_t sz
+  | output_buffer_420 => bits_t sz
+  | output_buffer_421 => bits_t sz
+  | output_buffer_422 => bits_t sz
+  | output_buffer_423 => bits_t sz
+  | output_buffer_424 => bits_t sz
+  | output_buffer_425 => bits_t sz
+  | output_buffer_426 => bits_t sz
+  | output_buffer_427 => bits_t sz
+  | output_buffer_428 => bits_t sz
+  | output_buffer_429 => bits_t sz
+  | output_buffer_430 => bits_t sz
+  | output_buffer_431 => bits_t sz
+  | output_buffer_432 => bits_t sz
+  | output_buffer_433 => bits_t sz
+  | output_buffer_434 => bits_t sz
+  | output_buffer_435 => bits_t sz
+  | output_buffer_436 => bits_t sz
+  | output_buffer_437 => bits_t sz
+  | output_buffer_438 => bits_t sz
+  | output_buffer_439 => bits_t sz
+  | output_buffer_440 => bits_t sz
+  | output_buffer_441 => bits_t sz
+  | output_buffer_442 => bits_t sz
+  | output_buffer_443 => bits_t sz
+  | output_buffer_444 => bits_t sz
+  | output_buffer_445 => bits_t sz
+  | output_buffer_446 => bits_t sz
+  | output_buffer_447 => bits_t sz
+  | output_buffer_448 => bits_t sz
+  | output_buffer_449 => bits_t sz
+  | output_buffer_450 => bits_t sz
+  | output_buffer_451 => bits_t sz
+  | output_buffer_452 => bits_t sz
+  | output_buffer_453 => bits_t sz
+  | output_buffer_454 => bits_t sz
+  | output_buffer_455 => bits_t sz
+  | output_buffer_456 => bits_t sz
+  | output_buffer_457 => bits_t sz
+  | output_buffer_458 => bits_t sz
+  | output_buffer_459 => bits_t sz
+  | output_buffer_460 => bits_t sz
+  | output_buffer_461 => bits_t sz
+  | output_buffer_462 => bits_t sz
+  | output_buffer_463 => bits_t sz
+  | output_buffer_464 => bits_t sz
+  | output_buffer_465 => bits_t sz
+  | output_buffer_466 => bits_t sz
+  | output_buffer_467 => bits_t sz
+  | output_buffer_468 => bits_t sz
+  | output_buffer_469 => bits_t sz
+  | output_buffer_470 => bits_t sz
+  | output_buffer_471 => bits_t sz
+  | output_buffer_472 => bits_t sz
+  | output_buffer_473 => bits_t sz
+  | output_buffer_474 => bits_t sz
+  | output_buffer_475 => bits_t sz
+  | output_buffer_476 => bits_t sz
+  | output_buffer_477 => bits_t sz
+  | output_buffer_478 => bits_t sz
+  | output_buffer_479 => bits_t sz
+  | output_buffer_480 => bits_t sz
+  | output_buffer_481 => bits_t sz
+  | output_buffer_482 => bits_t sz
+  | output_buffer_483 => bits_t sz
+  | output_buffer_484 => bits_t sz
+  | output_buffer_485 => bits_t sz
+  | output_buffer_486 => bits_t sz
+  | output_buffer_487 => bits_t sz
+  | output_buffer_488 => bits_t sz
+  | output_buffer_489 => bits_t sz
+  | output_buffer_490 => bits_t sz
+  | output_buffer_491 => bits_t sz
+  | output_buffer_492 => bits_t sz
+  | output_buffer_493 => bits_t sz
+  | output_buffer_494 => bits_t sz
+  | output_buffer_495 => bits_t sz
+  | output_buffer_496 => bits_t sz
+  | output_buffer_497 => bits_t sz
+  | output_buffer_498 => bits_t sz
+  | output_buffer_499 => bits_t sz
+  | output_buffer_500 => bits_t sz
+  | output_buffer_501 => bits_t sz
+  | output_buffer_502 => bits_t sz
+  | output_buffer_503 => bits_t sz
+  | output_buffer_504 => bits_t sz
+  | output_buffer_505 => bits_t sz
+  | output_buffer_506 => bits_t sz
+  | output_buffer_507 => bits_t sz
+  | output_buffer_508 => bits_t sz
+  | output_buffer_509 => bits_t sz
+  | output_buffer_510 => bits_t sz
+  | output_buffer_511 => bits_t sz
+  | output_buffer_512 => bits_t sz
+  | output_buffer_513 => bits_t sz
+  | output_buffer_514 => bits_t sz
+  | output_buffer_515 => bits_t sz
+  | output_buffer_516 => bits_t sz
+  | output_buffer_517 => bits_t sz
+  | output_buffer_518 => bits_t sz
+  | output_buffer_519 => bits_t sz
+  | output_buffer_520 => bits_t sz
+  | output_buffer_521 => bits_t sz
+  | output_buffer_522 => bits_t sz
+  | output_buffer_523 => bits_t sz
+  | output_buffer_524 => bits_t sz
+  | output_buffer_525 => bits_t sz
+  | output_buffer_526 => bits_t sz
+  | output_buffer_527 => bits_t sz
+  | output_buffer_528 => bits_t sz
+  | output_buffer_529 => bits_t sz
+  | output_buffer_530 => bits_t sz
+  | output_buffer_531 => bits_t sz
+  | output_buffer_532 => bits_t sz
+  | output_buffer_533 => bits_t sz
+  | output_buffer_534 => bits_t sz
+  | output_buffer_535 => bits_t sz
+  | output_buffer_536 => bits_t sz
   end.
 
 Inductive ext_fn_t :=
@@ -56,7 +1129,9 @@ Definition Sigma (fn: ext_fn_t) : ExternalSignature :=
 Then we declare the rules of the system.  Notice how ``doG`` writes at port 0 and ``doF`` reads at port 1.  This is because we're building a pipelined queue, not a bypassing one, so we expect clients to pull first and push second.  Notice also that each rule is "guarded" by a call to ``fail``; that is, if ``doF`` can't push into the queue because ``doG`` is lagging then ``doF`` won't run at all, and if there's no data ready for ``doG`` to consume because ``doF`` isn't keeping up then ``doG`` won't run.
 |*)
 
-Definition _doF : uaction _ _ :=
+Arguments Var {pos_t var_t fn_name_t reg_t ext_fn_t R Sigma sig} k {tau m}
+: assert.
+Definition _doF : uaction reg_t ext_fn_t :=
   {{
      let v := read0(input_buffer) in
      write0(input_buffer, extcall NextInput(v));
@@ -120,8 +1195,551 @@ Definition r : ContextEnv.(env_t) R :=
   #{ input_buffer  => Bits.of_nat 32 1;
      queue_empty   => Ob~1;
      queue_data    => Bits.of_nat 32 0;
-     output_buffer => Bits.of_nat 32 0 }#.
+     output_buffer => Bits.of_nat 32 0;
+     output_buffer_1 => Bits.of_nat 32 0;
+     output_buffer_2 => Bits.of_nat 32 0;
+     output_buffer_3 => Bits.of_nat 32 0;
+     output_buffer_4 => Bits.of_nat 32 0;
+     output_buffer_5 => Bits.of_nat 32 0;
+     output_buffer_6 => Bits.of_nat 32 0;
+     output_buffer_7 => Bits.of_nat 32 0;
+     output_buffer_8 => Bits.of_nat 32 0;
+     output_buffer_9 => Bits.of_nat 32 0;
+     output_buffer_10 => Bits.of_nat 32 0;
+     output_buffer_11 => Bits.of_nat 32 0;
+     output_buffer_12 => Bits.of_nat 32 0;
+     output_buffer_13 => Bits.of_nat 32 0;
+     output_buffer_14 => Bits.of_nat 32 0;
+     output_buffer_15 => Bits.of_nat 32 0;
+     output_buffer_16 => Bits.of_nat 32 0;
+     output_buffer_17 => Bits.of_nat 32 0;
+     output_buffer_18 => Bits.of_nat 32 0;
+     output_buffer_19 => Bits.of_nat 32 0;
+     output_buffer_20 => Bits.of_nat 32 0;
+     output_buffer_21 => Bits.of_nat 32 0;
+     output_buffer_22 => Bits.of_nat 32 0;
+     output_buffer_23 => Bits.of_nat 32 0;
+     output_buffer_24 => Bits.of_nat 32 0;
+     output_buffer_25 => Bits.of_nat 32 0;
+     output_buffer_26 => Bits.of_nat 32 0;
+     output_buffer_27 => Bits.of_nat 32 0;
+     output_buffer_28 => Bits.of_nat 32 0;
+     output_buffer_29 => Bits.of_nat 32 0;
+     output_buffer_30 => Bits.of_nat 32 0;
+     output_buffer_31 => Bits.of_nat 32 0;
+     output_buffer_32 => Bits.of_nat 32 0;
+     output_buffer_33 => Bits.of_nat 32 0;
+     output_buffer_34 => Bits.of_nat 32 0;
+     output_buffer_35 => Bits.of_nat 32 0;
+     output_buffer_36 => Bits.of_nat 32 0;
+     output_buffer_37 => Bits.of_nat 32 0;
+     output_buffer_38 => Bits.of_nat 32 0;
+     output_buffer_39 => Bits.of_nat 32 0;
+     output_buffer_40 => Bits.of_nat 32 0;
+     output_buffer_41 => Bits.of_nat 32 0;
+     output_buffer_42 => Bits.of_nat 32 0;
+     output_buffer_43 => Bits.of_nat 32 0;
+     output_buffer_44 => Bits.of_nat 32 0;
+     output_buffer_45 => Bits.of_nat 32 0;
+     output_buffer_46 => Bits.of_nat 32 0;
+     output_buffer_47 => Bits.of_nat 32 0;
+     output_buffer_48 => Bits.of_nat 32 0;
+     output_buffer_49 => Bits.of_nat 32 0;
+     output_buffer_50 => Bits.of_nat 32 0;
+     output_buffer_51 => Bits.of_nat 32 0;
+     output_buffer_52 => Bits.of_nat 32 0;
+     output_buffer_53 => Bits.of_nat 32 0;
+     output_buffer_54 => Bits.of_nat 32 0;
+     output_buffer_55 => Bits.of_nat 32 0;
+     output_buffer_56 => Bits.of_nat 32 0;
+     output_buffer_57 => Bits.of_nat 32 0;
+     output_buffer_58 => Bits.of_nat 32 0;
+     output_buffer_59 => Bits.of_nat 32 0;
+     output_buffer_60 => Bits.of_nat 32 0;
+     output_buffer_61 => Bits.of_nat 32 0;
+     output_buffer_62 => Bits.of_nat 32 0;
+     output_buffer_63 => Bits.of_nat 32 0;
+     output_buffer_64 => Bits.of_nat 32 0;
+     output_buffer_65 => Bits.of_nat 32 0;
+     output_buffer_66 => Bits.of_nat 32 0;
+     output_buffer_67 => Bits.of_nat 32 0;
+     output_buffer_68 => Bits.of_nat 32 0;
+     output_buffer_69 => Bits.of_nat 32 0;
+     output_buffer_70 => Bits.of_nat 32 0;
+     output_buffer_71 => Bits.of_nat 32 0;
+     output_buffer_72 => Bits.of_nat 32 0;
+     output_buffer_73 => Bits.of_nat 32 0;
+     output_buffer_74 => Bits.of_nat 32 0;
+     output_buffer_75 => Bits.of_nat 32 0;
+     output_buffer_76 => Bits.of_nat 32 0;
+     output_buffer_77 => Bits.of_nat 32 0;
+     output_buffer_78 => Bits.of_nat 32 0;
+     output_buffer_79 => Bits.of_nat 32 0;
+     output_buffer_80 => Bits.of_nat 32 0;
+     output_buffer_81 => Bits.of_nat 32 0;
+     output_buffer_82 => Bits.of_nat 32 0;
+     output_buffer_83 => Bits.of_nat 32 0;
+     output_buffer_84 => Bits.of_nat 32 0;
+     output_buffer_85 => Bits.of_nat 32 0;
+     output_buffer_86 => Bits.of_nat 32 0;
+     output_buffer_87 => Bits.of_nat 32 0;
+     output_buffer_88 => Bits.of_nat 32 0;
+     output_buffer_89 => Bits.of_nat 32 0;
+     output_buffer_90 => Bits.of_nat 32 0;
+     output_buffer_91 => Bits.of_nat 32 0;
+     output_buffer_92 => Bits.of_nat 32 0;
+     output_buffer_93 => Bits.of_nat 32 0;
+     output_buffer_94 => Bits.of_nat 32 0;
+     output_buffer_95 => Bits.of_nat 32 0;
+     output_buffer_96 => Bits.of_nat 32 0;
+     output_buffer_97 => Bits.of_nat 32 0;
+     output_buffer_98 => Bits.of_nat 32 0;
+     output_buffer_99 => Bits.of_nat 32 0;
+     output_buffer_100 => Bits.of_nat 32 0;
+     output_buffer_101 => Bits.of_nat 32 0;
+     output_buffer_102 => Bits.of_nat 32 0;
+     output_buffer_103 => Bits.of_nat 32 0;
+     output_buffer_104 => Bits.of_nat 32 0;
+     output_buffer_105 => Bits.of_nat 32 0;
+     output_buffer_106 => Bits.of_nat 32 0;
+     output_buffer_107 => Bits.of_nat 32 0;
+     output_buffer_108 => Bits.of_nat 32 0;
+     output_buffer_109 => Bits.of_nat 32 0;
+     output_buffer_110 => Bits.of_nat 32 0;
+     output_buffer_111 => Bits.of_nat 32 0;
+     output_buffer_112 => Bits.of_nat 32 0;
+     output_buffer_113 => Bits.of_nat 32 0;
+     output_buffer_114 => Bits.of_nat 32 0;
+     output_buffer_115 => Bits.of_nat 32 0;
+     output_buffer_116 => Bits.of_nat 32 0;
+     output_buffer_117 => Bits.of_nat 32 0;
+     output_buffer_118 => Bits.of_nat 32 0;
+     output_buffer_119 => Bits.of_nat 32 0;
+     output_buffer_120 => Bits.of_nat 32 0;
+     output_buffer_121 => Bits.of_nat 32 0;
+     output_buffer_122 => Bits.of_nat 32 0;
+     output_buffer_123 => Bits.of_nat 32 0;
+     output_buffer_124 => Bits.of_nat 32 0;
+     output_buffer_125 => Bits.of_nat 32 0;
+     output_buffer_126 => Bits.of_nat 32 0;
+     output_buffer_127 => Bits.of_nat 32 0;
+     output_buffer_128 => Bits.of_nat 32 0;
+     output_buffer_129 => Bits.of_nat 32 0;
+     output_buffer_130 => Bits.of_nat 32 0;
+     output_buffer_131 => Bits.of_nat 32 0;
+     output_buffer_132 => Bits.of_nat 32 0;
+     output_buffer_133 => Bits.of_nat 32 0;
+     output_buffer_134 => Bits.of_nat 32 0;
+     output_buffer_135 => Bits.of_nat 32 0;
+     output_buffer_136 => Bits.of_nat 32 0;
+     output_buffer_137 => Bits.of_nat 32 0;
+     output_buffer_138 => Bits.of_nat 32 0;
+     output_buffer_139 => Bits.of_nat 32 0;
+     output_buffer_140 => Bits.of_nat 32 0;
+     output_buffer_141 => Bits.of_nat 32 0;
+     output_buffer_142 => Bits.of_nat 32 0;
+     output_buffer_143 => Bits.of_nat 32 0;
+     output_buffer_144 => Bits.of_nat 32 0;
+     output_buffer_145 => Bits.of_nat 32 0;
+     output_buffer_146 => Bits.of_nat 32 0;
+     output_buffer_147 => Bits.of_nat 32 0;
+     output_buffer_148 => Bits.of_nat 32 0;
+     output_buffer_149 => Bits.of_nat 32 0;
+     output_buffer_150 => Bits.of_nat 32 0;
+     output_buffer_151 => Bits.of_nat 32 0;
+     output_buffer_152 => Bits.of_nat 32 0;
+     output_buffer_153 => Bits.of_nat 32 0;
+     output_buffer_154 => Bits.of_nat 32 0;
+     output_buffer_155 => Bits.of_nat 32 0;
+     output_buffer_156 => Bits.of_nat 32 0;
+     output_buffer_157 => Bits.of_nat 32 0;
+     output_buffer_158 => Bits.of_nat 32 0;
+     output_buffer_159 => Bits.of_nat 32 0;
+     output_buffer_160 => Bits.of_nat 32 0;
+     output_buffer_161 => Bits.of_nat 32 0;
+     output_buffer_162 => Bits.of_nat 32 0;
+     output_buffer_163 => Bits.of_nat 32 0;
+     output_buffer_164 => Bits.of_nat 32 0;
+     output_buffer_165 => Bits.of_nat 32 0;
+     output_buffer_166 => Bits.of_nat 32 0;
+     output_buffer_167 => Bits.of_nat 32 0;
+     output_buffer_168 => Bits.of_nat 32 0;
+     output_buffer_169 => Bits.of_nat 32 0;
+     output_buffer_170 => Bits.of_nat 32 0;
+     output_buffer_171 => Bits.of_nat 32 0;
+     output_buffer_172 => Bits.of_nat 32 0;
+     output_buffer_173 => Bits.of_nat 32 0;
+     output_buffer_174 => Bits.of_nat 32 0;
+     output_buffer_175 => Bits.of_nat 32 0;
+     output_buffer_176 => Bits.of_nat 32 0;
+     output_buffer_177 => Bits.of_nat 32 0;
+     output_buffer_178 => Bits.of_nat 32 0;
+     output_buffer_179 => Bits.of_nat 32 0;
+     output_buffer_180 => Bits.of_nat 32 0;
+     output_buffer_181 => Bits.of_nat 32 0;
+     output_buffer_182 => Bits.of_nat 32 0;
+     output_buffer_183 => Bits.of_nat 32 0;
+     output_buffer_184 => Bits.of_nat 32 0;
+     output_buffer_185 => Bits.of_nat 32 0;
+     output_buffer_186 => Bits.of_nat 32 0;
+     output_buffer_187 => Bits.of_nat 32 0;
+     output_buffer_188 => Bits.of_nat 32 0;
+     output_buffer_189 => Bits.of_nat 32 0;
+     output_buffer_190 => Bits.of_nat 32 0;
+     output_buffer_191 => Bits.of_nat 32 0;
+     output_buffer_192 => Bits.of_nat 32 0;
+     output_buffer_193 => Bits.of_nat 32 0;
+     output_buffer_194 => Bits.of_nat 32 0;
+     output_buffer_195 => Bits.of_nat 32 0;
+     output_buffer_196 => Bits.of_nat 32 0;
+     output_buffer_197 => Bits.of_nat 32 0;
+     output_buffer_198 => Bits.of_nat 32 0;
+     output_buffer_199 => Bits.of_nat 32 0;
+     output_buffer_200 => Bits.of_nat 32 0;
+     output_buffer_201 => Bits.of_nat 32 0;
+     output_buffer_202 => Bits.of_nat 32 0;
+     output_buffer_203 => Bits.of_nat 32 0;
+     output_buffer_204 => Bits.of_nat 32 0;
+     output_buffer_205 => Bits.of_nat 32 0;
+     output_buffer_206 => Bits.of_nat 32 0;
+     output_buffer_207 => Bits.of_nat 32 0;
+     output_buffer_208 => Bits.of_nat 32 0;
+     output_buffer_209 => Bits.of_nat 32 0;
+     output_buffer_210 => Bits.of_nat 32 0;
+     output_buffer_211 => Bits.of_nat 32 0;
+     output_buffer_212 => Bits.of_nat 32 0;
+     output_buffer_213 => Bits.of_nat 32 0;
+     output_buffer_214 => Bits.of_nat 32 0;
+     output_buffer_215 => Bits.of_nat 32 0;
+     output_buffer_216 => Bits.of_nat 32 0;
+     output_buffer_217 => Bits.of_nat 32 0;
+     output_buffer_218 => Bits.of_nat 32 0;
+     output_buffer_219 => Bits.of_nat 32 0;
+     output_buffer_220 => Bits.of_nat 32 0;
+     output_buffer_221 => Bits.of_nat 32 0;
+     output_buffer_222 => Bits.of_nat 32 0;
+     output_buffer_223 => Bits.of_nat 32 0;
+     output_buffer_224 => Bits.of_nat 32 0;
+     output_buffer_225 => Bits.of_nat 32 0;
+     output_buffer_226 => Bits.of_nat 32 0;
+     output_buffer_227 => Bits.of_nat 32 0;
+     output_buffer_228 => Bits.of_nat 32 0;
+     output_buffer_229 => Bits.of_nat 32 0;
+     output_buffer_230 => Bits.of_nat 32 0;
+     output_buffer_231 => Bits.of_nat 32 0;
+     output_buffer_232 => Bits.of_nat 32 0;
+     output_buffer_233 => Bits.of_nat 32 0;
+     output_buffer_234 => Bits.of_nat 32 0;
+     output_buffer_235 => Bits.of_nat 32 0;
+     output_buffer_236 => Bits.of_nat 32 0;
+     output_buffer_237 => Bits.of_nat 32 0;
+     output_buffer_238 => Bits.of_nat 32 0;
+     output_buffer_239 => Bits.of_nat 32 0;
+     output_buffer_240 => Bits.of_nat 32 0;
+     output_buffer_241 => Bits.of_nat 32 0;
+     output_buffer_242 => Bits.of_nat 32 0;
+     output_buffer_243 => Bits.of_nat 32 0;
+     output_buffer_244 => Bits.of_nat 32 0;
+     output_buffer_245 => Bits.of_nat 32 0;
+     output_buffer_246 => Bits.of_nat 32 0;
+     output_buffer_247 => Bits.of_nat 32 0;
+     output_buffer_248 => Bits.of_nat 32 0;
+     output_buffer_249 => Bits.of_nat 32 0;
+     output_buffer_250 => Bits.of_nat 32 0;
+     output_buffer_251 => Bits.of_nat 32 0;
+     output_buffer_252 => Bits.of_nat 32 0;
+     output_buffer_253 => Bits.of_nat 32 0;
+     output_buffer_254 => Bits.of_nat 32 0;
+     output_buffer_255 => Bits.of_nat 32 0;
+     output_buffer_256 => Bits.of_nat 32 0;
+     output_buffer_257 => Bits.of_nat 32 0;
+     output_buffer_258 => Bits.of_nat 32 0;
+     output_buffer_259 => Bits.of_nat 32 0;
+     output_buffer_260 => Bits.of_nat 32 0;
+     output_buffer_261 => Bits.of_nat 32 0;
+     output_buffer_262 => Bits.of_nat 32 0;
+     output_buffer_263 => Bits.of_nat 32 0;
+     output_buffer_264 => Bits.of_nat 32 0;
+     output_buffer_265 => Bits.of_nat 32 0;
+     output_buffer_266 => Bits.of_nat 32 0;
+     output_buffer_267 => Bits.of_nat 32 0;
+     output_buffer_268 => Bits.of_nat 32 0;
+     output_buffer_269 => Bits.of_nat 32 0;
+     output_buffer_270 => Bits.of_nat 32 0;
+     output_buffer_271 => Bits.of_nat 32 0;
+     output_buffer_272 => Bits.of_nat 32 0;
+     output_buffer_273 => Bits.of_nat 32 0;
+     output_buffer_274 => Bits.of_nat 32 0;
+     output_buffer_275 => Bits.of_nat 32 0;
+     output_buffer_276 => Bits.of_nat 32 0;
+     output_buffer_277 => Bits.of_nat 32 0;
+     output_buffer_278 => Bits.of_nat 32 0;
+     output_buffer_279 => Bits.of_nat 32 0;
+     output_buffer_280 => Bits.of_nat 32 0;
+     output_buffer_281 => Bits.of_nat 32 0;
+     output_buffer_282 => Bits.of_nat 32 0;
+     output_buffer_283 => Bits.of_nat 32 0;
+     output_buffer_284 => Bits.of_nat 32 0;
+     output_buffer_285 => Bits.of_nat 32 0;
+     output_buffer_286 => Bits.of_nat 32 0;
+     output_buffer_287 => Bits.of_nat 32 0;
+     output_buffer_288 => Bits.of_nat 32 0;
+     output_buffer_289 => Bits.of_nat 32 0;
+     output_buffer_290 => Bits.of_nat 32 0;
+     output_buffer_291 => Bits.of_nat 32 0;
+     output_buffer_292 => Bits.of_nat 32 0;
+     output_buffer_293 => Bits.of_nat 32 0;
+     output_buffer_294 => Bits.of_nat 32 0;
+     output_buffer_295 => Bits.of_nat 32 0;
+     output_buffer_296 => Bits.of_nat 32 0;
+     output_buffer_297 => Bits.of_nat 32 0;
+     output_buffer_298 => Bits.of_nat 32 0;
+     output_buffer_299 => Bits.of_nat 32 0;
+     output_buffer_300 => Bits.of_nat 32 0;
+     output_buffer_301 => Bits.of_nat 32 0;
+     output_buffer_302 => Bits.of_nat 32 0;
+     output_buffer_303 => Bits.of_nat 32 0;
+     output_buffer_304 => Bits.of_nat 32 0;
+     output_buffer_305 => Bits.of_nat 32 0;
+     output_buffer_306 => Bits.of_nat 32 0;
+     output_buffer_307 => Bits.of_nat 32 0;
+     output_buffer_308 => Bits.of_nat 32 0;
+     output_buffer_309 => Bits.of_nat 32 0;
+     output_buffer_310 => Bits.of_nat 32 0;
+     output_buffer_311 => Bits.of_nat 32 0;
+     output_buffer_312 => Bits.of_nat 32 0;
+     output_buffer_313 => Bits.of_nat 32 0;
+     output_buffer_314 => Bits.of_nat 32 0;
+     output_buffer_315 => Bits.of_nat 32 0;
+     output_buffer_316 => Bits.of_nat 32 0;
+     output_buffer_317 => Bits.of_nat 32 0;
+     output_buffer_318 => Bits.of_nat 32 0;
+     output_buffer_319 => Bits.of_nat 32 0;
+     output_buffer_320 => Bits.of_nat 32 0;
+     output_buffer_321 => Bits.of_nat 32 0;
+     output_buffer_322 => Bits.of_nat 32 0;
+     output_buffer_323 => Bits.of_nat 32 0;
+     output_buffer_324 => Bits.of_nat 32 0;
+     output_buffer_325 => Bits.of_nat 32 0;
+     output_buffer_326 => Bits.of_nat 32 0;
+     output_buffer_327 => Bits.of_nat 32 0;
+     output_buffer_328 => Bits.of_nat 32 0;
+     output_buffer_329 => Bits.of_nat 32 0;
+     output_buffer_330 => Bits.of_nat 32 0;
+     output_buffer_331 => Bits.of_nat 32 0;
+     output_buffer_332 => Bits.of_nat 32 0;
+     output_buffer_333 => Bits.of_nat 32 0;
+     output_buffer_334 => Bits.of_nat 32 0;
+     output_buffer_335 => Bits.of_nat 32 0;
+     output_buffer_336 => Bits.of_nat 32 0;
+     output_buffer_337 => Bits.of_nat 32 0;
+     output_buffer_338 => Bits.of_nat 32 0;
+     output_buffer_339 => Bits.of_nat 32 0;
+     output_buffer_340 => Bits.of_nat 32 0;
+     output_buffer_341 => Bits.of_nat 32 0;
+     output_buffer_342 => Bits.of_nat 32 0;
+     output_buffer_343 => Bits.of_nat 32 0;
+     output_buffer_344 => Bits.of_nat 32 0;
+     output_buffer_345 => Bits.of_nat 32 0;
+     output_buffer_346 => Bits.of_nat 32 0;
+     output_buffer_347 => Bits.of_nat 32 0;
+     output_buffer_348 => Bits.of_nat 32 0;
+     output_buffer_349 => Bits.of_nat 32 0;
+     output_buffer_350 => Bits.of_nat 32 0;
+     output_buffer_351 => Bits.of_nat 32 0;
+     output_buffer_352 => Bits.of_nat 32 0;
+     output_buffer_353 => Bits.of_nat 32 0;
+     output_buffer_354 => Bits.of_nat 32 0;
+     output_buffer_355 => Bits.of_nat 32 0;
+     output_buffer_356 => Bits.of_nat 32 0;
+     output_buffer_357 => Bits.of_nat 32 0;
+     output_buffer_358 => Bits.of_nat 32 0;
+     output_buffer_359 => Bits.of_nat 32 0;
+     output_buffer_360 => Bits.of_nat 32 0;
+     output_buffer_361 => Bits.of_nat 32 0;
+     output_buffer_362 => Bits.of_nat 32 0;
+     output_buffer_363 => Bits.of_nat 32 0;
+     output_buffer_364 => Bits.of_nat 32 0;
+     output_buffer_365 => Bits.of_nat 32 0;
+     output_buffer_366 => Bits.of_nat 32 0;
+     output_buffer_367 => Bits.of_nat 32 0;
+     output_buffer_368 => Bits.of_nat 32 0;
+     output_buffer_369 => Bits.of_nat 32 0;
+     output_buffer_370 => Bits.of_nat 32 0;
+     output_buffer_371 => Bits.of_nat 32 0;
+     output_buffer_372 => Bits.of_nat 32 0;
+     output_buffer_373 => Bits.of_nat 32 0;
+     output_buffer_374 => Bits.of_nat 32 0;
+     output_buffer_375 => Bits.of_nat 32 0;
+     output_buffer_376 => Bits.of_nat 32 0;
+     output_buffer_377 => Bits.of_nat 32 0;
+     output_buffer_378 => Bits.of_nat 32 0;
+     output_buffer_379 => Bits.of_nat 32 0;
+     output_buffer_380 => Bits.of_nat 32 0;
+     output_buffer_381 => Bits.of_nat 32 0;
+     output_buffer_382 => Bits.of_nat 32 0;
+     output_buffer_383 => Bits.of_nat 32 0;
+     output_buffer_384 => Bits.of_nat 32 0;
+     output_buffer_385 => Bits.of_nat 32 0;
+     output_buffer_386 => Bits.of_nat 32 0;
+     output_buffer_387 => Bits.of_nat 32 0;
+     output_buffer_388 => Bits.of_nat 32 0;
+     output_buffer_389 => Bits.of_nat 32 0;
+     output_buffer_390 => Bits.of_nat 32 0;
+     output_buffer_391 => Bits.of_nat 32 0;
+     output_buffer_392 => Bits.of_nat 32 0;
+     output_buffer_393 => Bits.of_nat 32 0;
+     output_buffer_394 => Bits.of_nat 32 0;
+     output_buffer_395 => Bits.of_nat 32 0;
+     output_buffer_396 => Bits.of_nat 32 0;
+     output_buffer_397 => Bits.of_nat 32 0;
+     output_buffer_398 => Bits.of_nat 32 0;
+     output_buffer_399 => Bits.of_nat 32 0;
+     output_buffer_400 => Bits.of_nat 32 0;
+     output_buffer_401 => Bits.of_nat 32 0;
+     output_buffer_402 => Bits.of_nat 32 0;
+     output_buffer_403 => Bits.of_nat 32 0;
+     output_buffer_404 => Bits.of_nat 32 0;
+     output_buffer_405 => Bits.of_nat 32 0;
+     output_buffer_406 => Bits.of_nat 32 0;
+     output_buffer_407 => Bits.of_nat 32 0;
+     output_buffer_408 => Bits.of_nat 32 0;
+     output_buffer_409 => Bits.of_nat 32 0;
+     output_buffer_410 => Bits.of_nat 32 0;
+     output_buffer_411 => Bits.of_nat 32 0;
+     output_buffer_412 => Bits.of_nat 32 0;
+     output_buffer_413 => Bits.of_nat 32 0;
+     output_buffer_414 => Bits.of_nat 32 0;
+     output_buffer_415 => Bits.of_nat 32 0;
+     output_buffer_416 => Bits.of_nat 32 0;
+     output_buffer_417 => Bits.of_nat 32 0;
+     output_buffer_418 => Bits.of_nat 32 0;
+     output_buffer_419 => Bits.of_nat 32 0;
+     output_buffer_420 => Bits.of_nat 32 0;
+     output_buffer_421 => Bits.of_nat 32 0;
+     output_buffer_422 => Bits.of_nat 32 0;
+     output_buffer_423 => Bits.of_nat 32 0;
+     output_buffer_424 => Bits.of_nat 32 0;
+     output_buffer_425 => Bits.of_nat 32 0;
+     output_buffer_426 => Bits.of_nat 32 0;
+     output_buffer_427 => Bits.of_nat 32 0;
+     output_buffer_428 => Bits.of_nat 32 0;
+     output_buffer_429 => Bits.of_nat 32 0;
+     output_buffer_430 => Bits.of_nat 32 0;
+     output_buffer_431 => Bits.of_nat 32 0;
+     output_buffer_432 => Bits.of_nat 32 0;
+     output_buffer_433 => Bits.of_nat 32 0;
+     output_buffer_434 => Bits.of_nat 32 0;
+     output_buffer_435 => Bits.of_nat 32 0;
+     output_buffer_436 => Bits.of_nat 32 0;
+     output_buffer_437 => Bits.of_nat 32 0;
+     output_buffer_438 => Bits.of_nat 32 0;
+     output_buffer_439 => Bits.of_nat 32 0;
+     output_buffer_440 => Bits.of_nat 32 0;
+     output_buffer_441 => Bits.of_nat 32 0;
+     output_buffer_442 => Bits.of_nat 32 0;
+     output_buffer_443 => Bits.of_nat 32 0;
+     output_buffer_444 => Bits.of_nat 32 0;
+     output_buffer_445 => Bits.of_nat 32 0;
+     output_buffer_446 => Bits.of_nat 32 0;
+     output_buffer_447 => Bits.of_nat 32 0;
+     output_buffer_448 => Bits.of_nat 32 0;
+     output_buffer_449 => Bits.of_nat 32 0;
+     output_buffer_450 => Bits.of_nat 32 0;
+     output_buffer_451 => Bits.of_nat 32 0;
+     output_buffer_452 => Bits.of_nat 32 0;
+     output_buffer_453 => Bits.of_nat 32 0;
+     output_buffer_454 => Bits.of_nat 32 0;
+     output_buffer_455 => Bits.of_nat 32 0;
+     output_buffer_456 => Bits.of_nat 32 0;
+     output_buffer_457 => Bits.of_nat 32 0;
+     output_buffer_458 => Bits.of_nat 32 0;
+     output_buffer_459 => Bits.of_nat 32 0;
+     output_buffer_460 => Bits.of_nat 32 0;
+     output_buffer_461 => Bits.of_nat 32 0;
+     output_buffer_462 => Bits.of_nat 32 0;
+     output_buffer_463 => Bits.of_nat 32 0;
+     output_buffer_464 => Bits.of_nat 32 0;
+     output_buffer_465 => Bits.of_nat 32 0;
+     output_buffer_466 => Bits.of_nat 32 0;
+     output_buffer_467 => Bits.of_nat 32 0;
+     output_buffer_468 => Bits.of_nat 32 0;
+     output_buffer_469 => Bits.of_nat 32 0;
+     output_buffer_470 => Bits.of_nat 32 0;
+     output_buffer_471 => Bits.of_nat 32 0;
+     output_buffer_472 => Bits.of_nat 32 0;
+     output_buffer_473 => Bits.of_nat 32 0;
+     output_buffer_474 => Bits.of_nat 32 0;
+     output_buffer_475 => Bits.of_nat 32 0;
+     output_buffer_476 => Bits.of_nat 32 0;
+     output_buffer_477 => Bits.of_nat 32 0;
+     output_buffer_478 => Bits.of_nat 32 0;
+     output_buffer_479 => Bits.of_nat 32 0;
+     output_buffer_480 => Bits.of_nat 32 0;
+     output_buffer_481 => Bits.of_nat 32 0;
+     output_buffer_482 => Bits.of_nat 32 0;
+     output_buffer_483 => Bits.of_nat 32 0;
+     output_buffer_484 => Bits.of_nat 32 0;
+     output_buffer_485 => Bits.of_nat 32 0;
+     output_buffer_486 => Bits.of_nat 32 0;
+     output_buffer_487 => Bits.of_nat 32 0;
+     output_buffer_488 => Bits.of_nat 32 0;
+     output_buffer_489 => Bits.of_nat 32 0;
+     output_buffer_490 => Bits.of_nat 32 0;
+     output_buffer_491 => Bits.of_nat 32 0;
+     output_buffer_492 => Bits.of_nat 32 0;
+     output_buffer_493 => Bits.of_nat 32 0;
+     output_buffer_494 => Bits.of_nat 32 0;
+     output_buffer_495 => Bits.of_nat 32 0;
+     output_buffer_496 => Bits.of_nat 32 0;
+     output_buffer_497 => Bits.of_nat 32 0;
+     output_buffer_498 => Bits.of_nat 32 0;
+     output_buffer_499 => Bits.of_nat 32 0;
+     output_buffer_500 => Bits.of_nat 32 0;
+     output_buffer_501 => Bits.of_nat 32 0;
+     output_buffer_502 => Bits.of_nat 32 0;
+     output_buffer_503 => Bits.of_nat 32 0;
+     output_buffer_504 => Bits.of_nat 32 0;
+     output_buffer_505 => Bits.of_nat 32 0;
+     output_buffer_506 => Bits.of_nat 32 0;
+     output_buffer_507 => Bits.of_nat 32 0;
+     output_buffer_508 => Bits.of_nat 32 0;
+     output_buffer_509 => Bits.of_nat 32 0;
+     output_buffer_510 => Bits.of_nat 32 0;
+     output_buffer_511 => Bits.of_nat 32 0;
+     output_buffer_512 => Bits.of_nat 32 0;
+     output_buffer_513 => Bits.of_nat 32 0;
+     output_buffer_514 => Bits.of_nat 32 0;
+     output_buffer_515 => Bits.of_nat 32 0;
+     output_buffer_516 => Bits.of_nat 32 0;
+     output_buffer_517 => Bits.of_nat 32 0;
+     output_buffer_518 => Bits.of_nat 32 0;
+     output_buffer_519 => Bits.of_nat 32 0;
+     output_buffer_520 => Bits.of_nat 32 0;
+     output_buffer_521 => Bits.of_nat 32 0;
+     output_buffer_522 => Bits.of_nat 32 0;
+     output_buffer_523 => Bits.of_nat 32 0;
+     output_buffer_524 => Bits.of_nat 32 0;
+     output_buffer_525 => Bits.of_nat 32 0;
+     output_buffer_526 => Bits.of_nat 32 0;
+     output_buffer_527 => Bits.of_nat 32 0;
+     output_buffer_528 => Bits.of_nat 32 0;
+     output_buffer_529 => Bits.of_nat 32 0;
+     output_buffer_530 => Bits.of_nat 32 0;
+     output_buffer_531 => Bits.of_nat 32 0;
+     output_buffer_532 => Bits.of_nat 32 0;
+     output_buffer_533 => Bits.of_nat 32 0;
+     output_buffer_534 => Bits.of_nat 32 0;
+     output_buffer_535 => Bits.of_nat 32 0;
+     output_buffer_536 => Bits.of_nat 32 0
+  }#.
 
+Require Import BitsToLists.
+Definition f_init := fun x => BitsToLists.val_of_value (r.[x]).
+Definition initial_context_env_val := ContextEnv.(create) (f_init).
+Time Compute initial_context_env_val.
+Print type.
+Time Compute @BitsToLists.val_of_value (bits_t 32000) (Bits.of_nat 32000 1).
 (*|
 For the external functions, we take something simple: ``f`` multiplies its input by 5, ``g`` adds one to its input, and ``next_input`` models the sequence of odd numbers ``1, 3, 5, 7, 9, …``:
 |*)
@@ -139,7 +1757,7 @@ In the first step of execution ``doG`` does not execute and ``doF`` reads 1 from
 The function ``interp_cycle`` computes this update: it returns a map of register values.
 |*)
 
-Compute (interp_cycle σ rules pipeline r). (* .unfold *)
+Compute (UntypedSemantics.interp_cycle σ rules pipeline r). (* .unfold *)
 
 (*|
 Here is an infinite stream capturing the initial state of the system and all snapshots of the system after each execution:
